theories/utils/Library_extra/Map_Extra.thy
@@ -93,4 +93,272 @@ lemma map_graph_list: "\<lbrakk>finite g; functional g\<rbrakk> \<Longrightarrow
   apply (auto dest:functional_listD)
 done
 
+definition map_inv :: "('a \<rightharpoonup> 'b) \<Rightarrow> ('b \<rightharpoonup> 'a)" where
+"map_inv f \<equiv> \<lambda> y. if (y \<in> ran f) then Some (SOME x. f x = Some y) else None"
+
+lemma map_inv_empty [simp]: "map_inv empty = empty"
+  by (simp add:map_inv_def)
+
+lemma map_inv_Some [simp]: "map_inv Some = Some"
+  by (simp add:map_inv_def ran_def)
+
+lemma map_inv_f_f [simp]: 
+  "\<lbrakk> inj_on f (dom f); f x = Some y \<rbrakk> \<Longrightarrow> map_inv f y = Some x"
+  apply (auto simp add: map_inv_def)
+  apply (rule some_equality)
+  apply (auto simp add:inj_on_def dom_def ran_def)
+done
+
+lemma dom_map_inv [simp]:
+  "dom (map_inv f) = ran f"
+  apply (auto simp add:map_inv_def)
+  apply (case_tac "x \<in> ran f")
+  apply (simp_all)
+done
+
+lemma ran_map_inv [simp]:
+  "inj_on f (dom f) \<Longrightarrow> ran (map_inv f) = dom f"
+  apply (auto simp add:map_inv_def ran_def)
+  apply (rule_tac x="a" in exI)
+  apply (force intro:someI)
+  apply (rule_tac x="y" in exI)
+  apply (auto)
+  apply (rule some_equality, simp_all)
+  apply (auto simp add:inj_on_def dom_def)
+done
+
+lemma dom_image_ran: "f ` dom f = Some ` ran f"
+  by (auto simp add:dom_def ran_def image_def)
+
+lemma inj_map_inv [intro]:
+  "inj_on f (dom f) \<Longrightarrow> inj_on (map_inv f) (ran f)"
+  apply (auto simp add:map_inv_def inj_on_def dom_def ran_def)
+  apply (frule_tac P="\<lambda> xa. f xa = Some x" in some_equality)
+  apply (auto)
+  apply (smt option.inject someI)
+done
+
+lemma inj_map_bij: "inj_on f (dom f) \<Longrightarrow> bij_betw f (dom f) (Some ` ran f)"
+  by (auto simp add:inj_on_def dom_def ran_def image_def bij_betw_def)
+
+lemma dom_left_map_add [simp]: "x \<in> dom g \<Longrightarrow> (f ++ g) x = g x"
+  by (auto simp add:map_add_def dom_def)
+
+lemma dom_right_map_add [simp]: "\<lbrakk> x \<notin> dom g; x \<in> dom f \<rbrakk> \<Longrightarrow> (f ++ g) x = f x"
+  by (auto simp add:map_add_def dom_def)
+
+lemma map_self_adjoin_complete [intro]: 
+  assumes "dom f \<inter> ran f = {}" "inj_on f (dom f)"
+  shows "inj_on (map_inv f ++ f) (dom f \<union> ran f)"
+  apply (rule inj_onI)
+  apply (insert assms)
+  apply (case_tac "x \<in> dom f")
+  apply (simp)
+  apply (case_tac "y \<in> dom f")
+  apply (simp add:inj_on_def)
+  apply (case_tac "y \<in> ran f")
+  apply (subgoal_tac "y \<in> dom (map_inv f)")
+  apply (simp)
+  apply (metis Int_iff domD empty_iff ranI ran_map_inv)
+  apply (simp)
+  apply (simp)
+  apply (simp)
+  apply (case_tac "y \<in> dom f")
+  apply (simp)
+  apply (case_tac "y \<in> ran f")
+  apply (subgoal_tac "y \<in> dom (map_inv f)")
+  apply (simp)
+  apply (metis Int_iff domD empty_iff ranI ran_map_inv)
+  apply (simp)
+  apply (metis Int_iff domD empty_iff ranI ran_map_inv)
+  apply (simp)
+  apply (metis (lifting) inj_map_inv inj_on_contraD)
+done
+
+lemma inj_completed_map [intro]:
+  "\<lbrakk> dom f = ran f; inj_on f (dom f) \<rbrakk> \<Longrightarrow> inj (Some ++ f)"
+  apply (drule inj_map_bij)
+  apply (auto simp add:bij_betw_def)
+  apply (auto simp add:inj_on_def)[1]
+  apply (case_tac "x \<in> dom f")
+  apply (simp)
+  apply (case_tac "y \<in> dom f")
+  apply (simp)
+  apply (simp add:ran_def)
+  apply (case_tac "y \<in> dom f")
+  apply (auto intro:ranI)
+done
+
+lemma bij_completed_map [intro]:
+  "\<lbrakk> dom f = ran f; inj_on f (dom f) \<rbrakk> \<Longrightarrow> 
+   bij_betw (Some ++ f) UNIV (range Some)"
+  apply (auto intro: inj_completed_map simp add:bij_betw_def)
+  apply (case_tac "xa \<in> dom f")
+  apply (simp)
+  apply (metis domD rangeI)
+  apply (simp)
+  apply (simp add:image_def)
+  apply (metis (full_types) dom_image_ran dom_left_map_add image_iff map_add_dom_app_simps(3))
+done
+
+lemma bij_map_Some:
+  "bij_betw f a (Some ` b) \<Longrightarrow> bij_betw (the \<circ> f) a b"
+  apply (auto simp add:bij_betw_def)
+  apply (smt comp_inj_on f_the_inv_into_f inj_on_def the.simps)
+  apply (smt image_iff the.simps)
+  apply (metis imageI image_compose the.simps)
+done
+
+lemma ran_map_add [simp]: 
+  "m`(dom m \<inter> dom n) = n`(dom m \<inter> dom n) \<Longrightarrow> 
+   ran(m++n) = ran n \<union> ran m"
+  apply (auto simp add:ran_def)
+  apply (metis map_add_find_right)
+  apply (case_tac "a \<in> dom n")
+  apply (subgoal_tac "\<exists> b. n b = Some x")
+  apply (auto)
+  apply (rule_tac x="b" in exI)
+  apply (simp)
+  apply (metis (hide_lams, no_types) IntI domI image_iff)
+  apply (metis (full_types) map_add_None map_add_dom_app_simps(1) map_add_dom_app_simps(3) not_None_eq)
+done
+
+lemma ran_maplets [simp]: 
+  "\<lbrakk> length xs = length ys; distinct xs \<rbrakk> \<Longrightarrow> ran [xs [\<mapsto>] ys] = set ys"
+    by (induct rule:list_induct2, simp_all)
+
+lemma inj_map_add:
+  "\<lbrakk> inj_on f (dom f); inj_on g (dom g); ran f \<inter> ran g = {} \<rbrakk> \<Longrightarrow> 
+   inj_on (f ++ g) (dom f \<union> dom g)"
+  apply (auto simp add:inj_on_def)
+  apply (smt disjoint_iff_not_equal domIff map_add_Some_iff map_add_dom_app_simps(1) ranI)
+  apply (metis domI)
+  apply (metis disjoint_iff_not_equal ranI)
+  apply (metis disjoint_iff_not_equal domIff map_add_Some_iff ranI)
+  apply (metis domI)
+done
+
+
+lemma map_inv_add [simp]:
+  assumes "inj_on f (dom f)" "inj_on g (dom g)" 
+          "dom f \<inter> dom g = {}" "ran f \<inter> ran g = {}" 
+  shows "map_inv (f ++ g) = map_inv f ++ map_inv g"
+proof (rule ext)
+
+  from assms have minj: "inj_on (f ++ g) (dom (f ++ g))"
+    by (simp, metis inj_map_add sup_commute)
+
+  fix x
+  have "x \<in> ran g \<Longrightarrow> map_inv (f ++ g) x = (map_inv f ++ map_inv g) x"
+  proof -
+    assume ran:"x \<in> ran g"
+    then obtain y where dom:"g y = Some x" "y \<in> dom g"
+      by (auto simp add:ran_def)
+
+    hence "(f ++ g) y = Some x"
+      by simp
+
+    with assms minj ran dom show "map_inv (f ++ g) x = (map_inv f ++ map_inv g) x"
+      by simp
+  qed
+
+  moreover have "\<lbrakk> x \<notin> ran g; x \<in> ran f \<rbrakk> \<Longrightarrow> map_inv (f ++ g) x = (map_inv f ++ map_inv g) x"
+  proof -
+    assume ran:"x \<notin> ran g" "x \<in> ran f"
+    with assms obtain y where dom:"f y = Some x" "y \<in> dom f" "y \<notin> dom g"
+      by (auto simp add:ran_def)
+
+    with ran have "(f ++ g) y = Some x"
+      by (simp)
+
+    with assms minj ran dom show "map_inv (f ++ g) x = (map_inv f ++ map_inv g) x"
+      by simp
+  qed
+
+  moreover from assms minj have "\<lbrakk> x \<notin> ran g; x \<notin> ran f \<rbrakk> \<Longrightarrow> map_inv (f ++ g) x = (map_inv f ++ map_inv g) x"
+
+    apply (auto simp add:map_inv_def ran_def map_add_def)
+    apply (metis dom_left_map_add map_add_def map_add_dom_app_simps(3))
+
+  done
+
+  ultimately show "map_inv (f ++ g) x = (map_inv f ++ map_inv g) x"
+    apply (case_tac "x \<in> ran g")
+    apply (simp)
+    apply (case_tac "x \<in> ran f")
+    apply (simp_all)
+  done
+qed
+
+lemma map_add_lookup [simp]: 
+  "x \<notin> dom f \<Longrightarrow> ([x \<mapsto> y] ++ f) x = Some y"
+  by (simp add:map_add_def dom_def)
+  
+lemma distinct_map_dom: 
+  "x \<notin> set xs \<Longrightarrow> x \<notin> dom [xs [\<mapsto>] ys]"
+  by (simp add:dom_def)
+
+lemma distinct_map_ran:
+  "\<lbrakk> distinct xs; y \<notin> set ys; length xs = length ys \<rbrakk> \<Longrightarrow> 
+   y \<notin> ran ([xs [\<mapsto>] ys])"
+  apply (simp add:map_upds_def)
+  apply (subgoal_tac "distinct (map fst (rev (zip xs ys)))")
+  apply (simp add:ran_distinct)
+  apply (metis (hide_lams, no_types) image_iff set_zip_rightD surjective_pairing)
+  apply (simp add:zip_rev[THEN sym])
+done
+
+lemma maplets_lookup[rule_format,dest]: 
+  "\<lbrakk> length xs = length ys; distinct xs \<rbrakk> \<Longrightarrow> 
+     \<forall> y. [xs [\<mapsto>] ys] x = Some y \<longrightarrow> y \<in> set ys"
+  by (induct rule:list_induct2, auto)
+
+lemma maplets_distinct_inj [intro]:
+  "\<lbrakk> length xs = length ys; distinct xs; distinct ys; set xs \<inter> set ys = {} \<rbrakk> \<Longrightarrow> 
+   inj_on [xs [\<mapsto>] ys] (set xs)"
+  apply (induct rule:list_induct2)
+  apply (simp_all)
+  apply (rule conjI)
+  apply (rule inj_onI)
+  apply (case_tac "xa = x")
+  apply (simp)
+  apply (case_tac "xa = y")
+  apply (simp)
+  apply (simp)
+  apply (case_tac "ya = x")
+  apply (simp)
+  apply (simp add:inj_on_def)
+  apply (auto)
+  apply (case_tac "xa = y")
+  apply (simp)
+  apply (metis maplets_lookup)
+done
+
+
+lemma map_inv_maplet[simp]: "map_inv [x \<mapsto> y] = [y \<mapsto> x]"
+  by (auto simp add:map_inv_def)
+
+lemma map_inv_maplets [simp]:
+  "\<lbrakk> length xs = length ys; distinct xs; distinct ys; set xs \<inter> set ys = {} \<rbrakk> \<Longrightarrow> 
+  map_inv [xs [\<mapsto>] ys] = [ys [\<mapsto>] xs]"
+  apply (induct rule:list_induct2)
+  apply (simp_all)
+  apply (subgoal_tac "map_inv ([xs [\<mapsto>] ys] ++ [x \<mapsto> y]) = map_inv [xs [\<mapsto>] ys] ++ map_inv [x \<mapsto> y]")
+  apply (simp)
+  apply (rule map_inv_add)
+  apply (auto)
+done
+  
+lemma maplets_lookup_nth [rule_format,simp]:
+  "\<lbrakk> length xs = length ys; distinct xs \<rbrakk> \<Longrightarrow> 
+   \<forall> i < length ys. [xs [\<mapsto>] ys] (xs ! i) = Some (ys ! i)"
+  apply (induct rule:list_induct2)
+  apply (auto)
+  apply (case_tac i)
+  apply (simp_all)
+  apply (metis nth_mem)
+  apply (case_tac i)
+  apply (auto)
+done
+
 end
